interface/App_new_ts.fsti
@@ -101,7 +101,7 @@ val merge_comm (l a b:concrete_st)
 val merge_idem (s:concrete_st)
   : Lemma (ensures eq (merge s s s) s)
 
-(*Two OP RC*)
+(*Two OP RCp*)
 //////////////// 
 val rc_ind_right (l a b:concrete_st) (o1 o2' o2:op_t)
   : Lemma (requires distinct_ops o1 o2 /\ Fst_then_snd? (rc o1 o2) /\
@@ -114,30 +114,33 @@ val rc_ind_left (l a b:concrete_st) (o1 o1' o2:op_t)
           (ensures eq (merge l (do (do a o1') o1) (do b o2)) (do (merge l (do (do a o1') o1) b) o2))
 
 //Special case of rc_intermediate_v1
-val rc_ind_lca (l:concrete_st) (o o1 o2:op_t)
-  : Lemma (requires distinct_ops o1 o2 /\ Fst_then_snd? (rc o1 o2) /\ distinct_ops o o1 /\ distinct_ops o o2 /\
+val rc_ind_lca (l:concrete_st) (ol o1 o2:op_t)
+  : Lemma (requires distinct_ops o1 o2 /\ Fst_then_snd? (rc o1 o2) /\ distinct_ops ol o1 /\ distinct_ops ol o2 /\
                     eq (merge l (do l o1) (do l o2)) (do (do l o1) o2))
-          (ensures eq (merge (do l o) (do (do l o) o1) (do (do l o) o2)) (do (do (do l o) o1) o2))
+          (ensures eq (merge (do l ol) (do (do l ol) o1) (do (do l ol) o2)) (do (do (do l ol) o1) o2))
 
 val rc_base (o1 o2:op_t)
   : Lemma (requires distinct_ops o1 o2 /\ Fst_then_snd? (rc o1 o2))
           (ensures eq (merge init_st (do init_st o1) (do init_st o2)) (do (do init_st o1) o2))
 
-val rc_inter_base_right (l s1 s2 s3:concrete_st) (o o' o1 o2:op_t) 
-  : Lemma (requires distinct_ops o o' /\ (Fst_then_snd? (rc o o') \/ (Ts_order? (rc o o') /\ fst o < fst o')) /\ 
+// because we proved that e_i^l rcp e is not possible. e_i^l is o' e is o here.
+//e_i^l vis e is not possible
+// so either e rcp e_i^l or e rct e_i^l is possible
+val rc_inter_base_right (l s1 s2 s3:concrete_st) (ob ol o1 o2:op_t) 
+  : Lemma (requires distinct_ops ob ol /\ (Fst_then_snd? (rc ob ol) \/ (Ts_order? (rc ob ol) (*/\ fst ob < fst ol*))) /\ 
                     distinct_ops o1 o2 /\ Fst_then_snd? (rc o1 o2) /\
-                    eq (merge (do l o') (do (do s1 o') o1) (do (do s2 o') o2)) (do (do (do s3 o') o1) o2) /\
+                    eq (merge (do l ol) (do (do s1 ol) o1) (do (do s2 ol) o2)) (do (do (do s3 ol) o1) o2) /\
                     eq (merge l (do s1 o1) (do s2 o2)) (do (do s3 o1) o2) /\
-                    eq (merge l (do s1 o') (do s2 o)) (do (do s3 o) o')) //***EXTRA***
-          (ensures eq (merge (do l o') (do (do s1 o') o1) (do (do (do s2 o) o') o2)) (do (do (do (do s3 o) o') o1) o2))
+                    eq (merge l (do s1 ol) (do s2 ob)) (do (do s3 ob) ol)) //***EXTRA***
+          (ensures eq (merge (do l ol) (do (do s1 ol) o1) (do (do (do s2 ob) ol) o2)) (do (do (do (do s3 ob) ol) o1) o2))
 
-val rc_inter_base_left (l s1 s2 s3:concrete_st) (o o' o1 o2:op_t) 
-  : Lemma (requires distinct_ops o o' /\ (Fst_then_snd? (rc o o') \/ (Ts_order? (rc o o') /\ fst o < fst o')) /\ 
+val rc_inter_base_left (l s1 s2 s3:concrete_st) (ob ol o1 o2:op_t) 
+  : Lemma (requires distinct_ops ob ol /\ (Fst_then_snd? (rc ob ol) \/ (Ts_order? (rc ob ol) (*/\ fst ob < fst ol*))) /\ 
                     distinct_ops o1 o2 /\ Fst_then_snd? (rc o1 o2) /\
-                    eq (merge (do l o') (do (do s1 o') o1) (do (do s2 o') o2)) (do (do (do s3 o') o1) o2) /\
+                    eq (merge (do l ol) (do (do s1 ol) o1) (do (do s2 ol) o2)) (do (do (do s3 ol) o1) o2) /\
                     eq (merge l (do s1 o1) (do s2 o2)) (do (do s3 o1) o2) /\
-                    eq (merge l (do s1 o) (do s2 o')) (do (do s3 o) o')) //***EXTRA***
-          (ensures eq (merge (do l o') (do (do (do s1 o) o') o1) (do (do s2 o') o2)) (do (do (do (do s3 o) o') o1) o2))
+                    eq (merge l (do s1 ob) (do s2 ol)) (do (do s3 ob) ol)) //***EXTRA***
+          (ensures eq (merge (do l ol) (do (do (do s1 ob) ol) o1) (do (do s2 ol) o2)) (do (do (do (do s3 ob) ol) o1) o2))
           
 (*val rc_intermediate_base_left_right (l s1 s2 s3:concrete_st) (o o' o1' o1 o2:op_t) 
   : Lemma (requires distinct_ops o o' /\ Fst_then_snd? (rc o o') /\  
@@ -147,32 +150,32 @@ val rc_inter_base_left (l s1 s2 s3:concrete_st) (o o' o1 o2:op_t)
                     eq (merge l (do s1 o1) (do s2 o2)) (do (do s3 o1) o2)) 
         (ensures eq (merge (do l o') (do (do (do s1 o1') o') o1) (do (do (do s2 o) o') o2)) (do (do (do (do (do s3 o1') o) o') o1) o2))*)
 
-val rc_inter_right (l s1 s2 s3:concrete_st) (o1 o2 o o' o_n:op_t)
+val rc_inter_right (l s1 s2 s3:concrete_st) (o1 o2 ob ol o:op_t)
   : Lemma (requires distinct_ops o1 o2 /\ Fst_then_snd? (rc o1 o2) /\  
-                    distinct_ops o o' /\ (Fst_then_snd? (rc o o') \/ (Ts_order? (rc o o') /\ fst o < fst o')) /\ 
-                    get_rid o_n <> get_rid o' (*o_n,o' must be concurrent*) /\
-                    ((~ (commutes_with o_n o)) \/ Fst_then_snd? (rc o_n o') \/ (Ts_order? (rc o_n o') /\ fst o_n < fst o')) /\
-                    eq (merge (do l o') (do (do s1 o') o1) (do (do (do s2 o) o') o2)) (do (do (do (do s3 o) o') o1) o2))
-      (ensures eq (merge (do l o') (do (do s1 o') o1) (do (do (do (do s2 o_n) o) o') o2)) (do (do (do (do (do s3 o_n) o) o') o1) o2)) 
+                    distinct_ops ob ol /\ (Fst_then_snd? (rc ob ol) \/ (Ts_order? (rc ob ol) (*/\ fst ob < fst ol*))) /\ 
+                    get_rid o <> get_rid ol (*o,ol must be concurrent*) /\
+                    ((~ (commutes_with o ob)) \/ Fst_then_snd? (rc o ol) \/ (Ts_order? (rc o ol) (*/\ fst o < fst ol*))) /\
+                    eq (merge (do l ol) (do (do s1 ol) o1) (do (do (do s2 ob) ol) o2)) (do (do (do (do s3 ob) ol) o1) o2))
+  (ensures eq (merge (do l ol) (do (do s1 ol) o1) (do (do (do (do s2 o) ob) ol) o2)) (do (do (do (do (do s3 o) ob) ol) o1) o2)) 
 
-val rc_inter_left (l s1 s2 s3:concrete_st) (o1 o2 o o' o_n:op_t)
+val rc_inter_left (l s1 s2 s3:concrete_st) (o1 o2 ob ol o:op_t)
   : Lemma (requires distinct_ops o1 o2 /\ Fst_then_snd? (rc o1 o2) /\  
-                    distinct_ops o o' /\ (Fst_then_snd? (rc o o') \/ (Ts_order? (rc o o') /\ fst o < fst o')) /\ 
-                    get_rid o_n <> get_rid o' (*o_n,o' must be concurrent*) /\
-                    ((~ (commutes_with o_n o)) \/ Fst_then_snd? (rc o_n o') \/ (Ts_order? (rc o_n o') /\ fst o_n < fst o')) /\
-                    eq (merge (do l o') (do (do (do s1 o) o') o1) (do (do s2 o') o2)) (do (do (do (do s3 o) o') o1) o2))
-      (ensures eq (merge (do l o') (do (do (do (do s1 o_n) o) o') o1) (do (do s2 o') o2)) (do (do (do (do (do s3 o_n) o) o') o1) o2))
+                    distinct_ops ob ol /\ (Fst_then_snd? (rc ob ol) \/ (Ts_order? (rc ob ol) (*/\ fst ob < fst ol*))) /\ 
+                    get_rid o <> get_rid ol (*o,ol must be concurrent*) /\
+                    ((~ (commutes_with o ob)) \/ Fst_then_snd? (rc o ol) \/ (Ts_order? (rc o ol) (*/\ fst o < fst ol*))) /\
+                    eq (merge (do l ol) (do (do (do s1 ob) ol) o1) (do (do s2 ol) o2)) (do (do (do (do s3 ob) ol) o1) o2))
+      (ensures eq (merge (do l ol) (do (do (do (do s1 o) ob) ol) o1) (do (do s2 ol) o2)) (do (do (do (do (do s3 o) ob) ol) o1) o2))
 
-// In general, the events o',o_n, below should be such that these exists o, (rc o o')
-val rc_inter_lca (l s1 s2 s3:concrete_st) (o1 o2 o' o_n:op_t)
+// In general, the events ol,oi, below should be such that these exists o, (rc o ol), (rc o oi)
+val rc_inter_lca (l s1 s2 s3:concrete_st) (o1 o2 ol oi:op_t)
   : Lemma (requires distinct_ops o1 o2 /\ Fst_then_snd? (rc o1 o2) /\ 
-                    (exists o. Fst_then_snd? (rc o o') \/ (Ts_order? (rc o o') /\ fst o < fst o')) /\ 
-                    (exists o. Fst_then_snd? (rc o o_n) \/ Ts_order? (rc o o_n) /\ fst o < fst o_n) /\ 
-                    eq (merge (do l o_n) (do (do s1 o_n) o1) (do (do s2 o_n) o2)) (do (do (do s3 o_n) o1) o2) /\
-                    eq (merge (do l o') (do (do s1 o') o1) (do (do s2 o') o2)) (do (do (do s3 o') o1) o2))
-    (ensures eq (merge (do (do l o_n) o') (do (do (do s1 o_n) o') o1) (do (do (do s2 o_n) o') o2)) (do (do (do (do s3 o_n) o') o1) o2))
+                    (exists o. Fst_then_snd? (rc o ol) \/ (Ts_order? (rc o ol) (*/\ fst o < fst ol*))) /\ 
+                    (exists o. Fst_then_snd? (rc o oi) \/ (Ts_order? (rc o oi) (*/\ fst o < fst oi*))) /\ 
+                    eq (merge (do l oi) (do (do s1 oi) o1) (do (do s2 oi) o2)) (do (do (do s3 oi) o1) o2) /\
+                    eq (merge (do l ol) (do (do s1 ol) o1) (do (do s2 ol) o2)) (do (do (do s3 ol) o1) o2))
+    (ensures eq (merge (do (do l oi) ol) (do (do (do s1 oi) ol) o1) (do (do (do s2 oi) ol) o2)) (do (do (do (do s3 oi) ol) o1) o2))
 
-(*Two OP TS_order*)
+(*Two OP RCt*)
 //////////////// 
 val ts_ind_right (l a b:concrete_st) (o1 o2' o2:op_t)
   : Lemma (requires distinct_ops o1 o2 /\ Ts_order? (rc o1 o2) /\ fst o1 < fst o2 /\
@@ -185,30 +188,30 @@ val ts_ind_left (l a b:concrete_st) (o1 o1' o2:op_t)
           (ensures eq (merge l (do (do a o1') o1) (do b o2)) (do (merge l (do (do a o1') o1) b) o2))
 
 //Special case of rc_intermediate_v1
-val ts_ind_lca (l:concrete_st) (o o1 o2:op_t)
-  : Lemma (requires distinct_ops o1 o2 /\ Ts_order? (rc o1 o2) /\ distinct_ops o o1 /\ distinct_ops o o2 /\ fst o1 < fst o2 /\
+val ts_ind_lca (l:concrete_st) (ol o1 o2:op_t)
+  : Lemma (requires distinct_ops o1 o2 /\ Ts_order? (rc o1 o2) /\ distinct_ops ol o1 /\ distinct_ops ol o2 /\ fst o1 < fst o2 /\
                     eq (merge l (do l o1) (do l o2)) (do (do l o1) o2))
-          (ensures eq (merge (do l o) (do (do l o) o1) (do (do l o) o2)) (do (do (do l o) o1) o2))
+          (ensures eq (merge (do l ol) (do (do l ol) o1) (do (do l ol) o2)) (do (do (do l ol) o1) o2))
 
 val ts_base (o1 o2:op_t)
   : Lemma (requires distinct_ops o1 o2 /\ Ts_order? (rc o1 o2) /\ fst o1 < fst o2)
           (ensures eq (merge init_st (do init_st o1) (do init_st o2)) (do (do init_st o1) o2))
 
-val ts_inter_base_right (l s1 s2 s3:concrete_st) (o o' o1 o2:op_t) 
-  : Lemma (requires distinct_ops o o' /\ (Fst_then_snd? (rc o o') \/ (Ts_order? (rc o o') /\ fst o < fst o')) /\ 
+val ts_inter_base_right (l s1 s2 s3:concrete_st) (ob ol o1 o2:op_t) 
+  : Lemma (requires distinct_ops ob ol /\ (Fst_then_snd? (rc ob ol) \/ (Ts_order? (rc ob ol) (*/\ fst ob < fst ol*))) /\ 
                     distinct_ops o1 o2 /\ Ts_order? (rc o1 o2) /\ fst o1 < fst o2 /\
-                    eq (merge (do l o') (do (do s1 o') o1) (do (do s2 o') o2)) (do (do (do s3 o') o1) o2) /\
+                    eq (merge (do l ol) (do (do s1 ol) o1) (do (do s2 ol) o2)) (do (do (do s3 ol) o1) o2) /\
                     eq (merge l (do s1 o1) (do s2 o2)) (do (do s3 o1) o2) /\
-                    eq (merge l (do s1 o') (do s2 o)) (do (do s3 o) o')) //***EXTRA***
-          (ensures eq (merge (do l o') (do (do s1 o') o1) (do (do (do s2 o) o') o2)) (do (do (do (do s3 o) o') o1) o2))
+                    eq (merge l (do s1 ol) (do s2 ob)) (do (do s3 ob) ol)) //***EXTRA***
+          (ensures eq (merge (do l ol) (do (do s1 ol) o1) (do (do (do s2 ob) ol) o2)) (do (do (do (do s3 ob) ol) o1) o2))
 
-val ts_inter_base_left (l s1 s2 s3:concrete_st) (o o' o1 o2:op_t) 
-  : Lemma (requires distinct_ops o o' /\ (Fst_then_snd? (rc o o') \/ (Ts_order? (rc o o') /\ fst o < fst o')) /\ 
+val ts_inter_base_left (l s1 s2 s3:concrete_st) (ob ol o1 o2:op_t) 
+  : Lemma (requires distinct_ops ob ol /\ (Fst_then_snd? (rc ob ol) \/ (Ts_order? (rc ob ol) (*/\ fst ob < fst ol*))) /\ 
                     distinct_ops o1 o2 /\ Ts_order? (rc o1 o2) /\ fst o1 < fst o2 /\
-                    eq (merge (do l o') (do (do s1 o') o1) (do (do s2 o') o2)) (do (do (do s3 o') o1) o2) /\
+                    eq (merge (do l ol) (do (do s1 ol) o1) (do (do s2 ol) o2)) (do (do (do s3 ol) o1) o2) /\
                     eq (merge l (do s1 o1) (do s2 o2)) (do (do s3 o1) o2) /\
-                    eq (merge l (do s1 o) (do s2 o')) (do (do s3 o) o')) //***EXTRA***
-          (ensures eq (merge (do l o') (do (do (do s1 o) o') o1) (do (do s2 o') o2)) (do (do (do (do s3 o) o') o1) o2))
+                    eq (merge l (do s1 ob) (do s2 ol)) (do (do s3 ob) ol)) //***EXTRA***
+          (ensures eq (merge (do l ol) (do (do (do s1 ob) ol) o1) (do (do s2 ol) o2)) (do (do (do (do s3 ob) ol) o1) o2))
           
 (*val rc_intermediate_base_left_right (l s1 s2 s3:concrete_st) (o o' o1' o1 o2:op_t) 
   : Lemma (requires distinct_ops o o' /\ Fst_then_snd? (rc o o') /\  
@@ -218,30 +221,30 @@ val ts_inter_base_left (l s1 s2 s3:concrete_st) (o o' o1 o2:op_t)
                     eq (merge l (do s1 o1) (do s2 o2)) (do (do s3 o1) o2)) 
         (ensures eq (merge (do l o') (do (do (do s1 o1') o') o1) (do (do (do s2 o) o') o2)) (do (do (do (do (do s3 o1') o) o') o1) o2))*)
 
-val ts_inter_right (l s1 s2 s3:concrete_st) (o1 o2 o o' o_n:op_t)
+val ts_inter_right (l s1 s2 s3:concrete_st) (o1 o2 ob ol o:op_t)
   : Lemma (requires distinct_ops o1 o2 /\ Ts_order? (rc o1 o2) /\ fst o1 < fst o2 /\
-                    distinct_ops o o' /\ (Fst_then_snd? (rc o o') \/ (Ts_order? (rc o o') /\ fst o < fst o')) /\ 
-                    get_rid o_n <> get_rid o' (*o_n,o' must be concurrent*) /\
-                    ((~ (commutes_with o_n o)) \/ Fst_then_snd? (rc o_n o') \/ (Ts_order? (rc o_n o') /\ fst o_n < fst o')) /\
-                    eq (merge (do l o') (do (do s1 o') o1) (do (do (do s2 o) o') o2)) (do (do (do (do s3 o) o') o1) o2))
-      (ensures eq (merge (do l o') (do (do s1 o') o1) (do (do (do (do s2 o_n) o) o') o2)) (do (do (do (do (do s3 o_n) o) o') o1) o2)) 
+                    distinct_ops ob ol /\ (Fst_then_snd? (rc ob ol) \/ (Ts_order? (rc ob ol) (*/\ fst ob < fst ol*))) /\ 
+                    get_rid o <> get_rid ol (*o,ol must be concurrent*) /\
+                    ((~ (commutes_with o ob)) \/ Fst_then_snd? (rc o ol) \/ (Ts_order? (rc o ol) (*/\ fst o < fst ol*))) /\
+                    eq (merge (do l ol) (do (do s1 ol) o1) (do (do (do s2 ob) ol) o2)) (do (do (do (do s3 ob) ol) o1) o2))
+      (ensures eq (merge (do l ol) (do (do s1 ol) o1) (do (do (do (do s2 o) ob) ol) o2)) (do (do (do (do (do s3 o) ob) ol) o1) o2)) 
 
-val ts_inter_left (l s1 s2 s3:concrete_st) (o1 o2 o o' o_n:op_t)
+val ts_inter_left (l s1 s2 s3:concrete_st) (o1 o2 ob ol o:op_t)
   : Lemma (requires distinct_ops o1 o2 /\ Ts_order? (rc o1 o2) /\ fst o1 < fst o2 /\ 
-                    distinct_ops o o' /\ (Fst_then_snd? (rc o o') \/ (Ts_order? (rc o o') /\ fst o < fst o')) /\ 
-                    get_rid o_n <> get_rid o' (*o_n,o' must be concurrent*) /\
-                    ((~ (commutes_with o_n o)) \/ Fst_then_snd? (rc o_n o') \/ (Ts_order? (rc o_n o') /\ fst o_n < fst o')) /\
-                    eq (merge (do l o') (do (do (do s1 o) o') o1) (do (do s2 o') o2)) (do (do (do (do s3 o) o') o1) o2))
-      (ensures eq (merge (do l o') (do (do (do (do s1 o_n) o) o') o1) (do (do s2 o') o2)) (do (do (do (do (do s3 o_n) o) o') o1) o2))
+                    distinct_ops ob ol /\ (Fst_then_snd? (rc ob ol) \/ (Ts_order? (rc ob ol) (*/\ fst ob < fst ol*))) /\ 
+                    get_rid o <> get_rid ol (*o,ol must be concurrent*) /\
+                    ((~ (commutes_with o ob)) \/ Fst_then_snd? (rc o ol) \/ (Ts_order? (rc o ol) (*/\ fst o < fst ol*))) /\
+                    eq (merge (do l ol) (do (do (do s1 ob) ol) o1) (do (do s2 ol) o2)) (do (do (do (do s3 ob) ol) o1) o2))
+      (ensures eq (merge (do l ol) (do (do (do (do s1 o) ob) ol) o1) (do (do s2 ol) o2)) (do (do (do (do (do s3 o) ob) ol) o1) o2))
 
-// In general, the events o',o_n, below should be such that these exists o, (rc o o')
-val ts_inter_lca (l s1 s2 s3:concrete_st) (o1 o2 o' o_n:op_t)
+// In general, the events ol,oi, below should be such that these exists o, (rc o ol), (rc o oi)
+val ts_inter_lca (l s1 s2 s3:concrete_st) (o1 o2 ol oi:op_t)
   : Lemma (requires distinct_ops o1 o2 /\ Ts_order? (rc o1 o2) /\ fst o1 < fst o2 /\
-                    (exists o. Fst_then_snd? (rc o o') \/ (Ts_order? (rc o o') /\ fst o < fst o')) /\ 
-                    (exists o. Fst_then_snd? (rc o o_n) \/ Ts_order? (rc o o_n) /\ fst o < fst o_n) /\ 
-                    eq (merge (do l o_n) (do (do s1 o_n) o1) (do (do s2 o_n) o2)) (do (do (do s3 o_n) o1) o2) /\
-                    eq (merge (do l o') (do (do s1 o') o1) (do (do s2 o') o2)) (do (do (do s3 o') o1) o2))
-    (ensures eq (merge (do (do l o_n) o') (do (do (do s1 o_n) o') o1) (do (do (do s2 o_n) o') o2)) (do (do (do (do s3 o_n) o') o1) o2))
+                    (exists o. Fst_then_snd? (rc o ol) \/ (Ts_order? (rc o ol) (*/\ fst o < fst ol*))) /\ 
+                    (exists o. Fst_then_snd? (rc o oi) \/ (Ts_order? (rc o oi) (*/\ fst o < fst oi*))) /\ 
+                    eq (merge (do l oi) (do (do s1 oi) o1) (do (do s2 oi) o2)) (do (do (do s3 oi) o1) o2) /\
+                    eq (merge (do l ol) (do (do s1 ol) o1) (do (do s2 ol) o2)) (do (do (do s3 ol) o1) o2))
+    (ensures eq (merge (do (do l oi) ol) (do (do (do s1 oi) ol) o1) (do (do (do s2 oi) ol) o2)) (do (do (do (do s3 oi) ol) o1) o2))
     
 (*One op*)
 ///////////////
@@ -249,19 +252,19 @@ val one_op_ind_right (l a b c:concrete_st) (o1 o1':op_t)
    : Lemma (requires eq (merge l a (do b o1)) (do (merge l a b) o1))
            (ensures eq (merge l a (do (do b o1') o1)) (do (merge l a (do b o1')) o1))
            
-val one_op_ind_lca (l:concrete_st) (o o1:op_t)
-  : Lemma (requires eq (merge l l (do l o1)) (do l o1) /\ fst o < fst o1)
-          (ensures eq (merge (do l o) (do l o) (do (do l o) o1)) (do (do l o) o1)) 
+val one_op_ind_lca (l:concrete_st) (ol o1:op_t)
+  : Lemma (requires eq (merge l l (do l o1)) (do l o1) /\ fst ol < fst o1)
+          (ensures eq (merge (do l ol) (do l ol) (do (do l ol) o1)) (do (do l ol) o1)) 
 
 val one_op_base (o1:op_t)
   : Lemma (ensures eq (merge init_st init_st (do init_st o1)) (do init_st o1))
 
-val one_op_inter_base_right (l s1 s2 s3:concrete_st) (o o' o1:op_t) 
-  : Lemma (requires distinct_ops o o' /\ (Fst_then_snd? (rc o o') \/ (Ts_order? (rc o o') /\ fst o < fst o')) /\ 
-                    eq (merge (do l o') (do s1 o') (do (do s2 o') o1)) (do (do s3 o') o1) /\
+val one_op_inter_base_right (l s1 s2 s3:concrete_st) (ob ol o1:op_t) 
+  : Lemma (requires distinct_ops ob ol /\ (Fst_then_snd? (rc ob ol) \/ (Ts_order? (rc ob ol) (*/\ fst ob < fst ol*))) /\ 
+                    eq (merge (do l ol) (do s1 ol) (do (do s2 ol) o1)) (do (do s3 ol) o1) /\
                     eq (merge l s1 (do s2 o1)) (do s3 o1) /\
-                    eq (merge l (do s1 o') (do s2 o)) (do (do s3 o) o')) //***EXTRA***
-          (ensures eq (merge (do l o') (do s1 o') (do (do (do s2 o) o') o1)) (do (do (do s3 o) o') o1))
+                    eq (merge l (do s1 ol) (do s2 ob)) (do (do s3 ob) ol)) //***EXTRA***
+          (ensures eq (merge (do l ol) (do s1 ol) (do (do (do s2 ob) ol) o1)) (do (do (do s3 ob) ol) o1))
 
 (*val intermediate_base_right_one_op_left (l s1 s2 s3:concrete_st) (o o' o1:op_t) 
   : Lemma (requires distinct_ops o o' /\ Fst_then_snd? (rc o o') /\ distinct_ops o' o1 /\
@@ -271,14 +274,14 @@ val one_op_inter_base_right (l s1 s2 s3:concrete_st) (o o' o1:op_t)
                     eq (merge l (do s1 o') (do s2 o)) (do (do s3 o) o')) //***EXTRA***
           (ensures eq (merge (do l o') (do (do s1 o') o1) (do (do s2 o) o')) (do (do (do s3 o) o') o1))*)
 
-val one_op_inter_base_left (l s1 s2 s3:concrete_st) (o o' o1:op_t) 
-  : Lemma (requires distinct_ops o o' /\ (Fst_then_snd? (rc o o') \/ (Ts_order? (rc o o') /\ fst o < fst o')) /\ 
-                    eq (merge (do l o') (do s1 o') (do (do s2 o') o1)) (do (do s3 o') o1) /\
-                    (Fst_then_snd? (rc o o1) ==> eq (merge l (do s1 o1) (do s2 o)) (do (merge l s1 (do s2 o)) o1)) /\ //***EXTRA***
+val one_op_inter_base_left (l s1 s2 s3:concrete_st) (ob ol o1:op_t) 
+  : Lemma (requires distinct_ops ob ol /\ (Fst_then_snd? (rc ob ol) \/ (Ts_order? (rc ob ol) (*/\ fst ob < fst ol*))) /\ 
+                    eq (merge (do l ol) (do s1 ol) (do (do s2 ol) o1)) (do (do s3 ol) o1) /\
+                    (Fst_then_snd? (rc ob o1) ==> eq (merge l (do s1 o1) (do s2 ob)) (do (merge l s1 (do s2 ob)) o1)) /\ //***EXTRA***
                     eq (merge l s1 (do s2 o1)) (do s3 o1) /\
-                    eq (merge l (do s1 o') (do s2 o)) (do (do s3 o) o') /\ //***EXTRA***
-                    eq (merge l (do (do s1 o) o') (do s2 o')) (do (do s3 o) o')) //***EXTRA***
-          (ensures eq (merge (do l o') (do (do s1 o) o') (do (do s2 o') o1)) (do (do (do s3 o) o') o1))
+                    eq (merge l (do s1 ol) (do s2 ob)) (do (do s3 ob) ol) /\ //***EXTRA***
+                    eq (merge l (do (do s1 ob) ol) (do s2 ol)) (do (do s3 ob) ol)) //***EXTRA***
+          (ensures eq (merge (do l ol) (do (do s1 ob) ol) (do (do s2 ol) o1)) (do (do (do s3 ob) ol) o1))
 
 (*val intermediate_base_left_right_one_op (l s1 s2 s3:concrete_st) (o o' o1' o1:op_t) 
   : Lemma (requires distinct_ops o o' /\ Fst_then_snd? (rc o o') /\
@@ -288,60 +291,66 @@ val one_op_inter_base_left (l s1 s2 s3:concrete_st) (o o' o1:op_t)
                     eq (merge l s1 (do s2 o1)) (do s3 o1))
           (ensures eq (merge (do l o') (do (do s1 o1') o') (do (do (do s2 o) o') o1)) (do (do (do (do s3 o1') o) o') o1))*)
 
-val one_op_inter_left (l s1 s2 s3:concrete_st) (o1 o o':op_t) (o_n:op_t{~ (commutes_with o_n o)})
-  : Lemma (requires distinct_ops o o' /\ (Fst_then_snd? (rc o o') \/ (Ts_order? (rc o o') /\ fst o < fst o')) /\ 
-                    get_rid o_n <> get_rid o' (*o_n,o' must be concurrent*) /\
-                    eq (merge (do l o') (do (do s1 o) o') (do (do s2 o') o1)) (do (do (do s3 o) o') o1))
-          (ensures eq (merge (do l o') (do (do (do s1 o_n) o) o') (do (do s2 o') o1)) (do (do (do (do s3 o_n) o) o') o1))
+val one_op_inter_left (l s1 s2 s3:concrete_st) (o1 ob ol:op_t) (o:op_t(*{~ (commutes_with o ob)}*))
+  : Lemma (requires distinct_ops ob ol /\ (Fst_then_snd? (rc ob ol) \/ (Ts_order? (rc ob ol) (*/\ fst ob < fst ol*))) /\ 
+                    get_rid o <> get_rid ol (*o,ol must be concurrent*) /\
+                    ((~ (commutes_with o ob)) \/ Fst_then_snd? (rc o ol) \/ (Ts_order? (rc o ol) (*/\ fst o < fst ol*))) /\
+                    eq (merge (do l ol) (do (do s1 ob) ol) (do (do s2 ol) o1)) (do (do (do s3 ob) ol) o1))
+          (ensures eq (merge (do l ol) (do (do (do s1 o) ob) ol) (do (do s2 ol) o1)) (do (do (do (do s3 o) ob) ol) o1))
 
-// In general, the events o',o_n, below should be such that these exists o, (rc o o')
-val one_op_inter_lca (l s1 s2 s3:concrete_st) (o1 o' o_n:op_t)
-  : Lemma (requires (exists o. Fst_then_snd? (rc o o') \/ (Ts_order? (rc o o') /\ fst o < fst o')) /\ 
-                    (exists o. Fst_then_snd? (rc o o_n) \/ (Ts_order? (rc o o_n) /\ fst o < fst o_n)) /\ 
-                    eq (merge (do l o_n) (do s1 o_n) (do (do s2 o_n) o1)) (do (do s3 o_n) o1) /\
-                    eq (merge (do l o') (do s1 o') (do (do s2 o') o1)) (do (do s3 o') o1))
-          (ensures eq (merge (do (do l o_n) o') (do (do s1 o_n) o') (do (do (do s2 o_n) o') o1)) (do (do (do s3 o_n) o') o1))
+// In general, the events ol,oi, below should be such that these exists o, (rc o ol), (rc o oi)
+val one_op_inter_lca (l s1 s2 s3:concrete_st) (o1 ol oi:op_t)
+  : Lemma (requires (exists o. Fst_then_snd? (rc o ol) \/ (Ts_order? (rc o ol) (*/\ fst o < fst ol*))) /\ 
+                    (exists o. Fst_then_snd? (rc o oi) \/ (Ts_order? (rc o oi) (*/\ fst o < fst oi*))) /\ 
+                    eq (merge (do l oi) (do s1 oi) (do (do s2 oi) o1)) (do (do s3 oi) o1) /\
+                    eq (merge (do l ol) (do s1 ol) (do (do s2 ol) o1)) (do (do s3 ol) o1))
+          (ensures eq (merge (do (do l oi) ol) (do (do s1 oi) ol) (do (do (do s2 oi) ol) o1)) (do (do (do s3 oi) ol) o1))
 
 (*Zero op *)
 ///////////////
-val zero_op_inter_base_right (l s1 s2 s3:concrete_st) (o o':op_t) 
-  : Lemma (requires distinct_ops o o' /\ (Fst_then_snd? (rc o o') \/ (Ts_order? (rc o o') /\ fst o < fst o')) /\ 
-                    eq (merge (do l o') (do s1 o') (do s2 o')) (do s3 o') /\
+// because we proved that e_i^l rcp eb is not possible.
+//e_i^l vis eb is not possible
+// so either eb rcp e_i^l or eb rct e_i^l is possible
+val zero_op_inter_base_right (l s1 s2 s3:concrete_st) (ob ol:op_t) 
+  : Lemma (requires distinct_ops ob ol /\ (Fst_then_snd? (rc ob ol) \/ (Ts_order? (rc ob ol) (*/\ fst ob < fst ol*))) /\ 
+                    eq (merge (do l ol) (do s1 ol) (do s2 ol)) (do s3 ol) /\
                     eq (merge l s1 s2) s3 /\
-                    eq (merge l (do s1 o') (do s2 o)) (do (do s3 o) o')) //***EXTRA***
-          (ensures eq (merge (do l o') (do s1 o') (do (do s2 o) o')) (do (do s3 o) o')) 
+                    eq (merge l (do s1 ol) (do s2 ob)) (do (do s3 ob) ol)) //***EXTRA***
+          (ensures eq (merge (do l ol) (do s1 ol) (do (do s2 ob) ol)) (do (do s3 ob) ol)) 
 
-val zero_op_inter_base_left (l s1 s2 s3:concrete_st) (o o' o1':op_t) 
-  : Lemma (requires distinct_ops o o' /\ (Fst_then_snd? (rc o o') \/ (Ts_order? (rc o o') /\ fst o < fst o')) /\ 
-                    distinct_ops o1' o' /\ (Fst_then_snd? (rc o1' o') \/ (Ts_order? (rc o1' o') /\ fst o1' < fst o')) /\ 
-                    eq (merge (do l o') (do s1 o') (do s2 o')) (do s3 o') /\
+val zero_op_inter_base_left (l s1 s2 s3:concrete_st) (ob ol o1':op_t) 
+  : Lemma (requires distinct_ops ob ol /\ (Fst_then_snd? (rc ob ol) \/ (Ts_order? (rc ob ol) (*/\ fst ob < fst ol*))) /\ 
+                    distinct_ops o1' ol /\ (Fst_then_snd? (rc o1' ol) \/ (Ts_order? (rc o1' ol) (*/\ fst o1' < fst ol*))) /\ 
+                    eq (merge (do l ol) (do s1 ol) (do s2 ol)) (do s3 ol) /\
                     eq (merge l s1 s2) s3) 
-          (ensures eq (merge (do l o') (do (do s1 o1') o') (do (do s2 o) o')) (do (do (do s3 o1') o) o'))
+          (ensures eq (merge (do l ol) (do (do s1 o1') ol) (do (do s2 ob) ol)) (do (do (do s3 o1') ob) ol))
 
-val zero_op_inter_right (l s1 s2 s3:concrete_st) (o o':op_t) (o_n:op_t{~ (commutes_with o_n o)})
-  : Lemma (requires distinct_ops o o' /\ (Fst_then_snd? (rc o o') \/ (Ts_order? (rc o o') /\ fst o < fst o')) /\ 
-                    get_rid o_n <> get_rid o' (*o_n,o' must be concurrent*) /\
-                    eq (merge (do l o') (do s1 o') (do (do s2 o) o')) (do (do s3 o) o'))
-          (ensures eq (merge (do l o') (do s1 o') (do (do (do s2 o_n) o) o')) (do (do (do s3 o_n) o) o')) 
+val zero_op_inter_right (l s1 s2 s3:concrete_st) (ob ol:op_t) (o:op_t(*{~ (commutes_with o ob)}*))
+  : Lemma (requires distinct_ops ob ol /\ (Fst_then_snd? (rc ob ol) \/ (Ts_order? (rc ob ol) (*/\ fst ob < fst ol*))) /\ 
+                    get_rid o <> get_rid ol (*o,ol must be concurrent*) /\
+                    ((~ (commutes_with o ob)) \/ Fst_then_snd? (rc o ol) \/ (Ts_order? (rc o ol) (*/\ fst o < fst ol*))) /\
+                    eq (merge (do l ol) (do s1 ol) (do (do s2 ob) ol)) (do (do s3 ob) ol))
+          (ensures eq (merge (do l ol) (do s1 ol) (do (do (do s2 o) ob) ol)) (do (do (do s3 o) ob) ol)) 
 
-val zero_op_inter_left (l s1 s2 s3:concrete_st) (o o':op_t) (o_n:op_t{~ (commutes_with o_n o)})
-  : Lemma (requires distinct_ops o o' /\ (Fst_then_snd? (rc o o') \/ (Ts_order? (rc o o') /\ fst o < fst o')) /\ 
-                    get_rid o_n <> get_rid o' (*o_n,o' must be concurrent*) /\
-                    eq (merge (do l o') (do (do s1 o) o') (do s2 o')) (do (do s3 o) o'))
-          (ensures eq (merge (do l o') (do (do (do s1 o_n) o) o') (do s2 o')) (do (do (do s3 o_n) o) o')) 
+val zero_op_inter_left (l s1 s2 s3:concrete_st) (ob ol:op_t) (o:op_t(*{~ (commutes_with o ob)}*))
+  : Lemma (requires distinct_ops ob ol /\ (Fst_then_snd? (rc ob ol) \/ (Ts_order? (rc ob ol) (*/\ fst ob < fst ol*))) /\ 
+                    get_rid o <> get_rid ol (*o_n,ol must be concurrent*) /\
+                    ((~ (commutes_with o ob)) \/ Fst_then_snd? (rc o ol) \/ (Ts_order? (rc o ol) (*/\ fst o < fst ol*))) /\
+                    eq (merge (do l ol) (do (do s1 ob) ol) (do s2 ol)) (do (do s3 ob) ol))
+          (ensures eq (merge (do l ol) (do (do (do s1 o) ob) ol) (do s2 ol)) (do (do (do s3 o) ob) ol)) 
 
-// In general, the event "o" below should be such that these exists o', (rc o' o)
-val zero_op_inter_lca_v1 (l s1 s2 s3:concrete_st) (o:op_t)
-  : Lemma (requires (exists o'. Fst_then_snd? (rc o' o) \/ (Ts_order? (rc o' o) /\ fst o' < fst o)) /\ eq (merge l s1 s2) s3)
-          (ensures eq (merge (do l o) (do s1 o) (do s2 o)) (do s3 o))
+// In general, the event "ol" below should be such that these exists o', (rc o' ol)
+val zero_op_inter_lca_v1 (l s1 s2 s3:concrete_st) (ol:op_t)
+  : Lemma (requires (exists o'. Fst_then_snd? (rc o' ol) \/ (Ts_order? (rc o' ol) (*/\ fst o' < fst ol*))) /\ eq (merge l s1 s2) s3)
+          (ensures eq (merge (do l ol) (do s1 ol) (do s2 ol)) (do s3 ol))
 
-// In general, the events o',o_n, below should be such that these exists o, (rc o o')
-val zero_op_inter_lca_v2 (l s1 s2 s3:concrete_st) (o' o_n:op_t)
-  : Lemma (requires (exists o. Fst_then_snd? (rc o o') \/ (Ts_order? (rc o o') /\ fst o < fst o')) /\ 
-                    (exists o. Fst_then_snd? (rc o o_n) \/ (Ts_order? (rc o o_n) /\ fst o < fst o_n)) /\
-                    eq (merge (do l o_n) (do s1 o_n) (do s2 o_n)) (do s3 o_n)  /\
-                    eq (merge (do l o') (do s1 o') (do s2 o')) (do s3 o'))
-          (ensures eq (merge (do (do l o_n) o') (do (do s1 o_n) o') (do (do s2 o_n) o')) (do (do s3 o_n) o'))
+// In general, the events ol,o_n, below should be such that these exists o, (rc o ol)
+val zero_op_inter_lca_v2 (l s1 s2 s3:concrete_st) (ol oi:op_t)
+  : Lemma (requires (exists o. Fst_then_snd? (rc o ol) \/ (Ts_order? (rc o ol) (*/\ fst o < fst ol*))) /\ 
+                    (exists o. Fst_then_snd? (rc o oi) \/ (Ts_order? (rc o oi) (*/\ fst o < fst oi*))) /\
+                    eq (merge (do l oi) (do s1 oi) (do s2 oi)) (do s3 oi)  /\
+                    eq (merge (do l ol) (do s1 ol) (do s2 ol)) (do s3 ol))
+          (ensures eq (merge (do (do l oi) ol) (do (do s1 oi) ol) (do (do s2 oi) ol)) (do (do s3 oi) ol))
 
 (* 2 op Comm  *)
 ///////////////////
@@ -366,24 +375,24 @@ val comm_ind_left (l a b c:concrete_st) (o1 o2' o2:op_t)
                     ~ (exists o3 b'. eq (do b o2) (do b' o3) /\ distinct_ops o1 o3 /\ Fst_then_snd? (rc o1 o3)))                    
           (ensures eq (merge l (do (do a o2') o1) (do b o2)) (do (do (merge l (do a o2') b) o2) o1))
 
-val comm_ind_lca (l:concrete_st) (o o1 o2:op_t)
-  : Lemma (requires distinct_ops o1 o2 /\ Either? (rc o1 o2) /\ distinct_ops o o1 /\ distinct_ops o o2 /\
+val comm_ind_lca (l:concrete_st) (ol o1 o2:op_t)
+  : Lemma (requires distinct_ops o1 o2 /\ Either? (rc o1 o2) /\ distinct_ops ol o1 /\ distinct_ops ol o2 /\
                     eq (merge l (do l o1) (do l o2)) (do (do l o2) o1))
-          (ensures eq (merge (do l o) (do (do l o) o1) (do (do l o) o2)) (do (do (do l o) o2) o1))
+          (ensures eq (merge (do l ol) (do (do l ol) o1) (do (do l ol) o2)) (do (do (do l ol) o2) o1))
 
 val comm_base (o1 o2:op_t)
   : Lemma (requires distinct_ops o1 o2 /\ Either? (rc o1 o2))
           (ensures eq (merge init_st (do init_st o1) (do init_st o2)) (do (do init_st o1) o2))
 
-val comm_inter_base_right (l s1 s2 s3:concrete_st) (o o' o1 o2:op_t) 
-  : Lemma (requires distinct_ops o o' /\ (Fst_then_snd? (rc o o') \/ (Ts_order? (rc o o') /\ fst o < fst o')) /\ 
+val comm_inter_base_right (l s1 s2 s3:concrete_st) (ob ol o1 o2:op_t) 
+  : Lemma (requires distinct_ops ob ol /\ (Fst_then_snd? (rc ob ol) \/ (Ts_order? (rc ob ol) (*/\ fst ob < fst ol*))) /\ 
                     distinct_ops o1 o2 /\ Either? (rc o1 o2) /\
-                    distinct_ops o' o1 /\ distinct_ops o' o2 /\
-                    eq (merge l (do s1 o1) (do (do s2 o) o2)) (do (do (merge l s1 (do s2 o)) o1) o2) /\ //comes from comm_ind_right
-                    eq (merge (do l o') (do (do s1 o') o1) (do (do s2 o') o2)) (do (do (do s3 o') o1) o2) /\ 
-                    eq (merge (do l o') (do s1 o') (do (do s2 o) o')) (do (do s3 o) o') /\ //comes from intermediate_base_zero_op
+                    distinct_ops ol o1 /\ distinct_ops ol o2 /\
+                    eq (merge l (do s1 o1) (do (do s2 ob) o2)) (do (do (merge l s1 (do s2 ob)) o1) o2) /\ //comes from comm_ind_right
+                    eq (merge (do l ol) (do (do s1 ol) o1) (do (do s2 ol) o2)) (do (do (do s3 ol) o1) o2) /\ 
+                    eq (merge (do l ol) (do s1 ol) (do (do s2 ob) ol)) (do (do s3 ob) ol) /\ //comes from intermediate_base_zero_op
                     eq (merge l (do s1 o1) (do s2 o2)) (do (do s3 o1) o2)) 
-          (ensures eq (merge (do l o') (do (do s1 o') o1) (do (do (do s2 o) o') o2)) (do (do (do (do s3 o) o') o1) o2))
+          (ensures eq (merge (do l ol) (do (do s1 ol) o1) (do (do (do s2 ob) ol) o2)) (do (do (do (do s3 ob) ol) o1) o2))
 
 (*val comm_inter_base_left_right (l s1 s2 s3:concrete_st) (o o' o1' o1 o2:op_t) 
   : Lemma (requires distinct_ops o o' /\ Fst_then_snd? (rc o o') /\ 
@@ -396,38 +405,37 @@ val comm_inter_base_right (l s1 s2 s3:concrete_st) (o o' o1 o2:op_t)
                     eq (merge (do l o') (do s1 o') (do (do s2 o) o')) (do (do s3 o) o')) //comes from intermediate_base_zero_op
         (ensures eq (merge (do l o') (do (do (do s1 o1') o') o1) (do (do (do s2 o) o') o2)) (do (do (do (do (do s3 o1') o) o') o1) o2))*) 
 
-val comm_inter_base_left (l s1 s2 s3:concrete_st) (o o' o1 o2:op_t) 
-  : Lemma (requires distinct_ops o o' /\ (Fst_then_snd? (rc o o') \/ (Ts_order? (rc o o') /\ fst o < fst o')) /\ 
+val comm_inter_base_left (l s1 s2 s3:concrete_st) (ob ol o1 o2:op_t) 
+  : Lemma (requires distinct_ops ob ol /\ (Fst_then_snd? (rc ob ol) \/ (Ts_order? (rc ob ol) (*/\ fst ob < fst ol*))) /\ 
                     distinct_ops o1 o2 /\ Either? (rc o1 o2) /\
-                    distinct_ops o' o1 /\ distinct_ops o' o2 /\
-                    eq (merge l (do (do s1 o) o1) (do s2 o2)) (do (do (merge l (do s1 o) s2) o1) o2) /\ //comes from comm_ind_left
-                    eq (merge (do l o') (do (do s1 o') o1) (do (do s2 o') o2)) (do (do (do s3 o') o1) o2) /\ 
-                    eq (merge (do l o') (do (do s1 o) o') (do s2 o')) (do (do s3 o) o') /\ //comes from intermediate_base_zero_op
+                    distinct_ops ol o1 /\ distinct_ops ol o2 /\
+                    eq (merge l (do (do s1 ob) o1) (do s2 o2)) (do (do (merge l (do s1 ob) s2) o1) o2) /\ //comes from comm_ind_left
+                    eq (merge (do l ol) (do (do s1 ol) o1) (do (do s2 ol) o2)) (do (do (do s3 ol) o1) o2) /\ 
+                    eq (merge (do l ol) (do (do s1 ob) ol) (do s2 ol)) (do (do s3 ob) ol) /\ //comes from intermediate_base_zero_op
                     eq (merge l (do s1 o1) (do s2 o2)) (do (do s3 o1) o2)) 
-          (ensures eq (merge (do l o') (do (do (do s1 o) o') o1) (do (do s2 o') o2)) (do (do (do (do s3 o) o') o1) o2))
+          (ensures eq (merge (do l ol) (do (do (do s1 ob) ol) o1) (do (do s2 ol) o2)) (do (do (do (do s3 ob) ol) o1) o2))
 
-val comm_inter_right (l s1 s2 s3:concrete_st) (o1 o2 o o':op_t) (o_n:op_t{~ (commutes_with o_n o)})
+val comm_inter_right (l s1 s2 s3:concrete_st) (o1 o2 ob ol:op_t) (o:op_t{~ (commutes_with o ob)})
   : Lemma (requires distinct_ops o1 o2 /\ Either? (rc o1 o2) /\  
-                    distinct_ops o o' /\ (Fst_then_snd? (rc o o') \/ (Ts_order? (rc o o') /\ fst o < fst o')) /\ 
-                    get_rid o_n <> get_rid o' (*o_n,o' must be concurrent*) /\
-                    distinct_ops o_n o' /\ Either? (rc o_n o') /\ 
-                    eq (merge (do l o') (do (do s1 o') o1) (do (do (do s2 o) o') o2)) (do (do (do (do s3 o) o') o1) o2))
-          (ensures eq (merge (do l o') (do (do s1 o') o1) (do (do (do (do s2 o_n) o) o') o2)) (do (do (do (do (do s3 o_n) o) o') o1) o2))
+                    distinct_ops ob ol /\ (Fst_then_snd? (rc ob ol) \/ (Ts_order? (rc ob ol) /\ fst ob < fst ol)) /\ 
+                    get_rid o <> get_rid ol (*o,ol must be concurrent*) /\
+                    distinct_ops o ol /\ Either? (rc o ol) /\ 
+                    eq (merge (do l ol) (do (do s1 ol) o1) (do (do (do s2 ob) ol) o2)) (do (do (do (do s3 ob) ol) o1) o2))
+          (ensures eq (merge (do l ol) (do (do s1 ol) o1) (do (do (do (do s2 o) ob) ol) o2)) (do (do (do (do (do s3 o) ob) ol) o1) o2))
 
-val comm_inter_left (l s1 s2 s3:concrete_st) (o1 o2 o o':op_t) (o_n:op_t{~ (commutes_with o_n o)})
+val comm_inter_left (l s1 s2 s3:concrete_st) (o1 o2 ob ol:op_t) (o:op_t{~ (commutes_with o ob)})
   : Lemma (requires distinct_ops o1 o2 /\ Either? (rc o1 o2) /\  
-                    distinct_ops o o' /\ (Fst_then_snd? (rc o o') \/ (Ts_order? (rc o o') /\ fst o < fst o')) /\ 
-                    get_rid o_n <> get_rid o' (*o_n,o' must be concurrent*) /\
-                    distinct_ops o_n o' /\ Either? (rc o_n o') /\ 
-                    //eq (merge (do l o') (do (do (do s1 o_n) o') o1) (do (do s2 o') o2)) (do (do (do (do s3 o_n) o') o1) o2) /\ //***EXTRA***
-                    eq (merge (do l o') (do (do (do s1 o) o') o1) (do (do s2 o') o2)) (do (do (do (do s3 o) o') o1) o2))
-          (ensures eq (merge (do l o') (do (do (do (do s1 o_n) o) o') o1) (do (do s2 o') o2)) (do (do (do (do (do s3 o_n) o) o') o1) o2))
+                    distinct_ops ob ol /\ (Fst_then_snd? (rc ob ol) \/ (Ts_order? (rc ob ol) /\ fst ob < fst ol)) /\ 
+                    get_rid o <> get_rid ol (*o,ol must be concurrent*) /\
+                    distinct_ops o ol /\ Either? (rc o ol) /\ 
+                    eq (merge (do l ol) (do (do (do s1 ob) ol) o1) (do (do s2 ol) o2)) (do (do (do (do s3 ob) ol) o1) o2))
+          (ensures eq (merge (do l ol) (do (do (do (do s1 o) ob) ol) o1) (do (do s2 ol) o2)) (do (do (do (do (do s3 o) ob) ol) o1) o2))
 
-val comm_inter_lca (l s1 s2 s3:concrete_st) (o1 o2 o:op_t)
-  : Lemma (requires distinct_ops o1 o2 /\ Either? (rc o1 o2) /\ distinct_ops o1 o /\ distinct_ops o o2 /\
-                    (exists o'. Fst_then_snd? (rc o' o) \/ (Ts_order? (rc o' o) /\ fst o' < fst o)) /\
+val comm_inter_lca (l s1 s2 s3:concrete_st) (o1 o2 ol:op_t)
+  : Lemma (requires distinct_ops o1 o2 /\ Either? (rc o1 o2) /\ distinct_ops ol o1 /\ distinct_ops ol o2 /\
+                    (exists o'. Fst_then_snd? (rc o' ol) \/ (Ts_order? (rc o' ol) (*/\ fst o' < fst ol*))) /\
                     eq (merge l (do s1 o1) (do s2 o2)) (do (do s3 o1) o2))
-          (ensures eq (merge (do l o) (do (do s1 o) o1) (do (do s2 o) o2)) (do (do (do s3 o) o1) o2))
+          (ensures eq (merge (do l ol) (do (do s1 ol) o1) (do (do s2 ol) o2)) (do (do (do s3 ol) o1) o2))
 
 ////////////////////////////////////////////////////////////////
 //// Sequential implementation //////
