mrdts-new/Map_eff/App_new_ts.fst
@@ -188,7 +188,7 @@ let rc_base' (o1 o2:op_t)
           (ensures eq (merge init_st (do init_st o1) (do init_st o2)) (do (do init_st o1) o2)) = ()
 
 let rc_inter_base_right' (l s1 s2 s3:concrete_st) (o o' o1 o2:op_t) 
-  : Lemma (requires distinct_ops o o' /\ (Fst_then_snd? (rc o o') \/ (Ts_order? (rc o o') /\ fst o < fst o')) /\
+  : Lemma (requires distinct_ops o o' /\ (Fst_then_snd? (rc o o') \/ (Ts_order? (rc o o') (*/\ fst o < fst o'*))) /\
                     distinct_ops o1 o2 /\ Fst_then_snd? (rc o1 o2) /\
                     eq (merge (do l o') (do (do s1 o') o1) (do (do s2 o') o2)) (do (do (do s3 o') o1) o2) /\
                     eq (merge l (do s1 o1) (do s2 o2)) (do (do s3 o1) o2) /\
@@ -200,7 +200,7 @@ let rc_inter_base_right' (l s1 s2 s3:concrete_st) (o o' o1 o2:op_t)
           (ensures eq (merge (do l o') (do (do s1 o') o1) (do (do (do s2 o) o') o2)) (do (do (do (do s3 o) o') o1) o2)) = ()
           
 let rc_inter_base_left' (l s1 s2 s3:concrete_st) (o o' o1 o2:op_t) 
-  : Lemma (requires distinct_ops o o' /\ (Fst_then_snd? (rc o o') \/ (Ts_order? (rc o o') /\ fst o < fst o')) /\
+  : Lemma (requires distinct_ops o o' /\ (Fst_then_snd? (rc o o') \/ (Ts_order? (rc o o') (*/\ fst o < fst o'*))) /\
                     distinct_ops o1 o2 /\ Fst_then_snd? (rc o1 o2) /\
                     eq (merge (do l o') (do (do s1 o') o1) (do (do s2 o') o2)) (do (do (do s3 o') o1) o2) /\
                     eq (merge l (do s1 o1) (do s2 o2)) (do (do s3 o1) o2) /\
@@ -213,9 +213,9 @@ let rc_inter_base_left' (l s1 s2 s3:concrete_st) (o o' o1 o2:op_t)
           
 let rc_inter_right' (l s1 s2 s3:concrete_st) (o1 o2 o o' o_n:op_t)
   : Lemma (requires distinct_ops o1 o2 /\ Fst_then_snd? (rc o1 o2) /\  
-                    distinct_ops o o' /\ (Fst_then_snd? (rc o o') \/ (Ts_order? (rc o o') /\ fst o < fst o')) /\
+                    distinct_ops o o' /\ (Fst_then_snd? (rc o o') \/ (Ts_order? (rc o o') (*/\ fst o < fst o'*))) /\
                     get_rid o_n <> get_rid o' (*o_n,o' must be concurrent*) /\
-                    ((~ (commutes_with o_n o)) \/ Fst_then_snd? (rc o_n o') \/ (Ts_order? (rc o_n o') /\ fst o_n < fst o')) /\
+                    ((~ (commutes_with o_n o)) \/ Fst_then_snd? (rc o_n o') \/ (Ts_order? (rc o_n o') (*/\ fst o_n < fst o'*))) /\
                     eq (merge (do l o') (do (do s1 o') o1) (do (do (do s2 o) o') o2)) (do (do (do (do s3 o) o') o1) o2) /\
                     (forall k. eq_l (fst (sel_k (merge (do l o') (do (do s1 o') o1) (do (do (do (do s2 o_n) o) o') o2)) k))
                                (fst (sel_k (do (do (do (do (do s3 o_n) o) o') o1) o2) k)) /\
@@ -225,9 +225,9 @@ let rc_inter_right' (l s1 s2 s3:concrete_st) (o1 o2 o o' o_n:op_t)
 
 let rc_inter_left' (l s1 s2 s3:concrete_st) (o1 o2 o o' o_n:op_t)
   : Lemma (requires distinct_ops o1 o2 /\ Fst_then_snd? (rc o1 o2) /\  
-                    distinct_ops o o' /\ (Fst_then_snd? (rc o o') \/ (Ts_order? (rc o o') /\ fst o < fst o')) /\ 
+                    distinct_ops o o' /\ (Fst_then_snd? (rc o o') \/ (Ts_order? (rc o o') (*/\ fst o < fst o'*))) /\ 
                     get_rid o_n <> get_rid o' (*o_n,o' must be concurrent*) /\
-                    ((~ (commutes_with o_n o)) \/ Fst_then_snd? (rc o_n o') \/ (Ts_order? (rc o_n o') /\ fst o_n < fst o')) /\
+                    ((~ (commutes_with o_n o)) \/ Fst_then_snd? (rc o_n o') \/ (Ts_order? (rc o_n o') (*/\ fst o_n < fst o'*))) /\
                     eq (merge (do l o') (do (do (do s1 o) o') o1) (do (do s2 o') o2)) (do (do (do (do s3 o) o') o1) o2) /\
                     (forall k. eq_l (fst (sel_k (merge (do l o') (do (do (do (do s1 o_n) o) o') o1) (do (do s2 o') o2)) k))
                                (fst (sel_k (do (do (do (do (do s3 o_n) o) o') o1) o2) k)) /\
@@ -237,8 +237,8 @@ let rc_inter_left' (l s1 s2 s3:concrete_st) (o1 o2 o o' o_n:op_t)
 
 let rc_inter_lca' (l s1 s2 s3:concrete_st) (o1 o2 o' o_n:op_t)
   : Lemma (requires distinct_ops o1 o2 /\ Fst_then_snd? (rc o1 o2) /\ 
-                    (exists o. Fst_then_snd? (rc o o') \/ (Ts_order? (rc o o') /\ fst o < fst o')) /\ 
-                    (exists o. Fst_then_snd? (rc o o_n) \/ Ts_order? (rc o o_n) /\ fst o < fst o_n) /\ 
+                    (exists o. Fst_then_snd? (rc o o') \/ (Ts_order? (rc o o') (*/\ fst o < fst o'*))) /\ 
+                    (exists o. Fst_then_snd? (rc o o_n) \/ (Ts_order? (rc o o_n) (*/\ fst o < fst o_n*))) /\ 
                     eq (merge (do l o_n) (do (do s1 o_n) o1) (do (do s2 o_n) o2)) (do (do (do s3 o_n) o1) o2) /\
                     eq (merge (do l o') (do (do s1 o') o1) (do (do s2 o') o2)) (do (do (do s3 o') o1) o2) /\
                     (forall k. eq_l (fst (sel_k (merge (do (do l o_n) o') (do (do (do s1 o_n) o') o1) (do (do (do s2 o_n) o') o2)) k))
@@ -282,7 +282,7 @@ let ts_base' (o1 o2:op_t)
           (ensures eq (merge init_st (do init_st o1) (do init_st o2)) (do (do init_st o1) o2)) = ()
 
 let ts_inter_base_right' (l s1 s2 s3:concrete_st) (o o' o1 o2:op_t) 
-  : Lemma (requires distinct_ops o o' /\ (Fst_then_snd? (rc o o') \/ (Ts_order? (rc o o') /\ fst o < fst o')) /\ 
+  : Lemma (requires distinct_ops o o' /\ (Fst_then_snd? (rc o o') \/ (Ts_order? (rc o o') (*/\ fst o < fst o'*))) /\ 
                     distinct_ops o1 o2 /\ Ts_order? (rc o1 o2) /\ fst o1 < fst o2 /\
                     eq (merge (do l o') (do (do s1 o') o1) (do (do s2 o') o2)) (do (do (do s3 o') o1) o2) /\
                     eq (merge l (do s1 o1) (do s2 o2)) (do (do s3 o1) o2) /\
@@ -294,7 +294,7 @@ let ts_inter_base_right' (l s1 s2 s3:concrete_st) (o o' o1 o2:op_t)
           (ensures eq (merge (do l o') (do (do s1 o') o1) (do (do (do s2 o) o') o2)) (do (do (do (do s3 o) o') o1) o2)) = ()
 
 let ts_inter_base_left' (l s1 s2 s3:concrete_st) (o o' o1 o2:op_t) 
-  : Lemma (requires distinct_ops o o' /\ (Fst_then_snd? (rc o o') \/ (Ts_order? (rc o o') /\ fst o < fst o')) /\ 
+  : Lemma (requires distinct_ops o o' /\ (Fst_then_snd? (rc o o') \/ (Ts_order? (rc o o') (*/\ fst o < fst o'*))) /\ 
                     distinct_ops o1 o2 /\ Ts_order? (rc o1 o2) /\ fst o1 < fst o2 /\
                     eq (merge (do l o') (do (do s1 o') o1) (do (do s2 o') o2)) (do (do (do s3 o') o1) o2) /\
                     eq (merge l (do s1 o1) (do s2 o2)) (do (do s3 o1) o2) /\
@@ -307,7 +307,7 @@ let ts_inter_base_left' (l s1 s2 s3:concrete_st) (o o' o1 o2:op_t)
 
 let ts_inter_right' (l s1 s2 s3:concrete_st) (o1 o2 o o' o_n:op_t)
   : Lemma (requires distinct_ops o1 o2 /\ Ts_order? (rc o1 o2) /\ fst o1 < fst o2 /\
-                    distinct_ops o o' /\ (Fst_then_snd? (rc o o') \/ (Ts_order? (rc o o') /\ fst o < fst o')) /\ 
+                    distinct_ops o o' /\ (Fst_then_snd? (rc o o') \/ (Ts_order? (rc o o') (*/\ fst o < fst o'*))) /\ 
                     get_rid o_n <> get_rid o' (*o_n,o' must be concurrent*) /\
                     ((~ (commutes_with o_n o)) \/ Fst_then_snd? (rc o_n o') \/ (Ts_order? (rc o_n o') /\ fst o_n < fst o')) /\
                     eq (merge (do l o') (do (do s1 o') o1) (do (do (do s2 o) o') o2)) (do (do (do (do s3 o) o') o1) o2) /\
@@ -319,9 +319,9 @@ let ts_inter_right' (l s1 s2 s3:concrete_st) (o1 o2 o o' o_n:op_t)
 
 let ts_inter_left' (l s1 s2 s3:concrete_st) (o1 o2 o o' o_n:op_t)
   : Lemma (requires distinct_ops o1 o2 /\ Ts_order? (rc o1 o2) /\ fst o1 < fst o2 /\ 
-                    distinct_ops o o' /\ (Fst_then_snd? (rc o o') \/ (Ts_order? (rc o o') /\ fst o < fst o')) /\ 
+                    distinct_ops o o' /\ (Fst_then_snd? (rc o o') \/ (Ts_order? (rc o o') (*/\ fst o < fst o'*))) /\ 
                     get_rid o_n <> get_rid o' (*o_n,o' must be concurrent*) /\
-                    ((~ (commutes_with o_n o)) \/ Fst_then_snd? (rc o_n o') \/ (Ts_order? (rc o_n o') /\ fst o_n < fst o')) /\
+                    ((~ (commutes_with o_n o)) \/ Fst_then_snd? (rc o_n o') \/ (Ts_order? (rc o_n o') (*/\ fst o_n < fst o'*))) /\
                     eq (merge (do l o') (do (do (do s1 o) o') o1) (do (do s2 o') o2)) (do (do (do (do s3 o) o') o1) o2) /\
                     (forall k. eq_l (fst (sel_k (merge (do l o') (do (do (do (do s1 o_n) o) o') o1) (do (do s2 o') o2)) k))
                                (fst (sel_k (do (do (do (do (do s3 o_n) o) o') o1) o2) k)) /\
@@ -332,8 +332,8 @@ let ts_inter_left' (l s1 s2 s3:concrete_st) (o1 o2 o o' o_n:op_t)
 // In general, the events o',o_n, below should be such that these exists o, (rc o o')
 let ts_inter_lca' (l s1 s2 s3:concrete_st) (o1 o2 o' o_n:op_t)
   : Lemma (requires distinct_ops o1 o2 /\ Ts_order? (rc o1 o2) /\ fst o1 < fst o2 /\
-                    (exists o. Fst_then_snd? (rc o o') \/ (Ts_order? (rc o o') /\ fst o < fst o')) /\ 
-                    (exists o. Fst_then_snd? (rc o o_n) \/ Ts_order? (rc o o_n) /\ fst o < fst o_n) /\ 
+                    (exists o. Fst_then_snd? (rc o o') \/ (Ts_order? (rc o o') (*/\ fst o < fst o'*))) /\ 
+                    (exists o. Fst_then_snd? (rc o o_n) \/ (Ts_order? (rc o o_n) (*/\ fst o < fst o_n*))) /\ 
                     eq (merge (do l o_n) (do (do s1 o_n) o1) (do (do s2 o_n) o2)) (do (do (do s3 o_n) o1) o2) /\
                     eq (merge (do l o') (do (do s1 o') o1) (do (do s2 o') o2)) (do (do (do s3 o') o1) o2) /\
                     (forall k. eq_l (fst (sel_k (merge (do (do l o_n) o') (do (do (do s1 o_n) o') o1) (do (do (do s2 o_n) o') o2))  k))
@@ -364,7 +364,7 @@ let one_op_base' (o1:op_t)
   : Lemma (ensures eq (merge init_st init_st (do init_st o1)) (do init_st o1)) = ()
 
 let one_op_inter_base_right' (l s1 s2 s3:concrete_st) (o o' o1:op_t) 
-  : Lemma (requires distinct_ops o o' /\ (Fst_then_snd? (rc o o') \/ (Ts_order? (rc o o') /\ fst o < fst o')) /\ 
+  : Lemma (requires distinct_ops o o' /\ (Fst_then_snd? (rc o o') \/ (Ts_order? (rc o o') (*/\ fst o < fst o'*))) /\ 
                     eq (merge (do l o') (do s1 o') (do (do s2 o') o1)) (do (do s3 o') o1) /\
                     eq (merge l s1 (do s2 o1)) (do s3 o1) /\
                     eq (merge l (do s1 o') (do s2 o)) (do (do s3 o) o') /\ //***EXTRA***
@@ -374,9 +374,10 @@ let one_op_inter_base_right' (l s1 s2 s3:concrete_st) (o o' o1:op_t)
                                (snd (sel_k (do (do (do s3 o) o') o1) k))))
           (ensures eq (merge (do l o') (do s1 o') (do (do (do s2 o) o') o1)) (do (do (do s3 o) o') o1)) = ()
 
-let one_op_inter_left' (l s1 s2 s3:concrete_st) (o1 o o':op_t) (o_n:op_t{~ (commutes_with o_n o)})
-  : Lemma (requires distinct_ops o o' /\ (Fst_then_snd? (rc o o') \/ (Ts_order? (rc o o') /\ fst o < fst o')) /\ 
+let one_op_inter_left' (l s1 s2 s3:concrete_st) (o1 o o':op_t) (o_n:op_t(*{~ (commutes_with o_n o)}*))
+  : Lemma (requires distinct_ops o o' /\ (Fst_then_snd? (rc o o') \/ (Ts_order? (rc o o') (*/\ fst o < fst o'*))) /\ 
                     get_rid o_n <> get_rid o' (*o_n,o' must be concurrent*) /\
+                    ((~ (commutes_with o_n o)) \/ Fst_then_snd? (rc o_n o') \/ (Ts_order? (rc o_n o') (*/\ fst o_n < fst o'*))) /\
                     eq (merge (do l o') (do (do s1 o) o') (do (do s2 o') o1)) (do (do (do s3 o) o') o1) /\
                     (forall k. eq_l (fst (sel_k (merge (do l o') (do (do (do s1 o_n) o) o') (do (do s2 o') o1)) k))
                                (fst (sel_k (do (do (do (do s3 o_n) o) o') o1) k)) /\
@@ -385,8 +386,8 @@ let one_op_inter_left' (l s1 s2 s3:concrete_st) (o1 o o':op_t) (o_n:op_t{~ (comm
           (ensures eq (merge (do l o') (do (do (do s1 o_n) o) o') (do (do s2 o') o1)) (do (do (do (do s3 o_n) o) o') o1)) = ()
 
 let one_op_inter_lca' (l s1 s2 s3:concrete_st) (o1 o' o_n:op_t)
-  : Lemma (requires (exists o. Fst_then_snd? (rc o o') \/ (Ts_order? (rc o o') /\ fst o < fst o')) /\ 
-                    (exists o. Fst_then_snd? (rc o o_n) \/ (Ts_order? (rc o o_n) /\ fst o < fst o_n)) /\ 
+  : Lemma (requires (exists o. Fst_then_snd? (rc o o') \/ (Ts_order? (rc o o') (*/\ fst o < fst o'*))) /\ 
+                    (exists o. Fst_then_snd? (rc o o_n) \/ (Ts_order? (rc o o_n) (*/\ fst o < fst o_n*))) /\ 
                     eq (merge (do l o_n) (do s1 o_n) (do (do s2 o_n) o1)) (do (do s3 o_n) o1) /\
                     eq (merge (do l o') (do s1 o') (do (do s2 o') o1)) (do (do s3 o') o1) /\
                     (forall k. eq_l (fst (sel_k (merge (do (do l o_n) o') (do (do s1 o_n) o') (do (do (do s2 o_n) o') o1)) k))
@@ -398,7 +399,7 @@ let one_op_inter_lca' (l s1 s2 s3:concrete_st) (o1 o' o_n:op_t)
 (*Zero op *)
 ///////////////
 let zero_op_inter_base_right' (l s1 s2 s3:concrete_st) (o o':op_t) 
-  : Lemma (requires distinct_ops o o' /\ (Fst_then_snd? (rc o o') \/ (Ts_order? (rc o o') /\ fst o < fst o')) /\ 
+  : Lemma (requires distinct_ops o o' /\ (Fst_then_snd? (rc o o') \/ (Ts_order? (rc o o') (*/\ fst o < fst o'*))) /\ 
                     eq (merge (do l o') (do s1 o') (do s2 o')) (do s3 o') /\
                     eq (merge l s1 s2) s3 /\
                     eq (merge l (do s1 o') (do s2 o)) (do (do s3 o) o') /\ //***EXTRA***
@@ -409,8 +410,8 @@ let zero_op_inter_base_right' (l s1 s2 s3:concrete_st) (o o':op_t)
           (ensures eq (merge (do l o') (do s1 o') (do (do s2 o) o')) (do (do s3 o) o')) = ()
 
 let zero_op_inter_base_left' (l s1 s2 s3:concrete_st) (o o' o1':op_t) 
-  : Lemma (requires distinct_ops o o' /\ (Fst_then_snd? (rc o o') \/ (Ts_order? (rc o o') /\ fst o < fst o')) /\ 
-                    distinct_ops o1' o' /\ (Fst_then_snd? (rc o1' o') \/ (Ts_order? (rc o1' o') /\ fst o1' < fst o')) /\ 
+  : Lemma (requires distinct_ops o o' /\ (Fst_then_snd? (rc o o') \/ (Ts_order? (rc o o') (*/\ fst o < fst o'*))) /\ 
+                    distinct_ops o1' o' /\ (Fst_then_snd? (rc o1' o') \/ (Ts_order? (rc o1' o') (*/\ fst o1' < fst o'*))) /\ 
                     eq (merge (do l o') (do s1 o') (do s2 o')) (do s3 o') /\
                     eq (merge l s1 s2) s3 /\
                     (forall k. eq_l (fst (sel_k (merge (do l o') (do (do s1 o1') o') (do (do s2 o) o')) k))
@@ -419,9 +420,10 @@ let zero_op_inter_base_left' (l s1 s2 s3:concrete_st) (o o' o1':op_t)
                                (snd (sel_k (do (do (do s3 o1') o) o') k)))) 
           (ensures eq (merge (do l o') (do (do s1 o1') o') (do (do s2 o) o')) (do (do (do s3 o1') o) o')) = ()
 
-let zero_op_inter_right' (l s1 s2 s3:concrete_st) (o o':op_t) (o_n:op_t{~ (commutes_with o_n o)})
-  : Lemma (requires distinct_ops o o' /\ (Fst_then_snd? (rc o o') \/ (Ts_order? (rc o o') /\ fst o < fst o')) /\ 
+let zero_op_inter_right' (l s1 s2 s3:concrete_st) (o o':op_t) (o_n:op_t(*{~ (commutes_with o_n o)}*))
+  : Lemma (requires distinct_ops o o' /\ (Fst_then_snd? (rc o o') \/ (Ts_order? (rc o o') (*/\ fst o < fst o'*))) /\ 
                     get_rid o_n <> get_rid o' (*o_n,o' must be concurrent*) /\
+                    ((~ (commutes_with o_n o)) \/ Fst_then_snd? (rc o_n o') \/ (Ts_order? (rc o_n o') (*/\ fst o_n < fst o'*))) /\
                     eq (merge (do l o') (do s1 o') (do (do s2 o) o')) (do (do s3 o) o') /\
                     (forall k. eq_l (fst (sel_k (merge (do l o') (do s1 o') (do (do (do s2 o_n) o) o'))k))
                                (fst (sel_k (do (do (do s3 o_n) o) o') k)) /\
@@ -429,9 +431,10 @@ let zero_op_inter_right' (l s1 s2 s3:concrete_st) (o o':op_t) (o_n:op_t{~ (commu
                                (snd (sel_k (do (do (do s3 o_n) o) o') k)))) 
           (ensures eq (merge (do l o') (do s1 o') (do (do (do s2 o_n) o) o')) (do (do (do s3 o_n) o) o')) = ()
 
-let zero_op_inter_left' (l s1 s2 s3:concrete_st) (o o':op_t) (o_n:op_t{~ (commutes_with o_n o)})
-  : Lemma (requires distinct_ops o o' /\ (Fst_then_snd? (rc o o') \/ (Ts_order? (rc o o') /\ fst o < fst o')) /\ 
+let zero_op_inter_left' (l s1 s2 s3:concrete_st) (o o':op_t) (o_n:op_t(*{~ (commutes_with o_n o)}*))
+  : Lemma (requires distinct_ops o o' /\ (Fst_then_snd? (rc o o') \/ (Ts_order? (rc o o') (*/\ fst o < fst o'*))) /\ 
                     get_rid o_n <> get_rid o' (*o_n,o' must be concurrent*) /\
+                    ((~ (commutes_with o_n o)) \/ Fst_then_snd? (rc o_n o') \/ (Ts_order? (rc o_n o') (*/\ fst o_n < fst o'*))) /\
                     eq (merge (do l o') (do (do s1 o) o') (do s2 o')) (do (do s3 o) o') /\
                     (forall k. eq_l (fst (sel_k (merge (do l o') (do (do (do s1 o_n) o) o') (do s2 o')) k))
                                (fst (sel_k (do (do (do s3 o_n) o) o') k)) /\
@@ -441,7 +444,7 @@ let zero_op_inter_left' (l s1 s2 s3:concrete_st) (o o':op_t) (o_n:op_t{~ (commut
 
 // In general, the event "o" below should be such that these exists o', (rc o' o)
 let zero_op_inter_lca_v1' (l s1 s2 s3:concrete_st) (o:op_t)
-  : Lemma (requires (exists o'. Fst_then_snd? (rc o' o) \/ (Ts_order? (rc o' o) /\ fst o' < fst o)) /\ eq (merge l s1 s2) s3 /\
+  : Lemma (requires (exists o'. Fst_then_snd? (rc o' o) \/ (Ts_order? (rc o' o) (*/\ fst o' < fst o*))) /\ eq (merge l s1 s2) s3 /\
                     (forall k. eq_l (fst (sel_k (merge (do l o) (do s1 o) (do s2 o)) k))
                                (fst (sel_k (do s3 o) k)) /\
                           eq_e (snd (sel_k (merge (do l o) (do s1 o) (do s2 o)) k))
@@ -450,8 +453,8 @@ let zero_op_inter_lca_v1' (l s1 s2 s3:concrete_st) (o:op_t)
 
 // In general, the events o',o_n, below should be such that these exists o, (rc o o')
 let zero_op_inter_lca_v2' (l s1 s2 s3:concrete_st) (o' o_n:op_t)
-  : Lemma (requires (exists o. Fst_then_snd? (rc o o') \/ (Ts_order? (rc o o') /\ fst o < fst o')) /\ 
-                    (exists o. Fst_then_snd? (rc o o_n) \/ (Ts_order? (rc o o_n) /\ fst o < fst o_n)) /\
+  : Lemma (requires (exists o. Fst_then_snd? (rc o o') \/ (Ts_order? (rc o o') (*/\ fst o < fst o'*))) /\ 
+                    (exists o. Fst_then_snd? (rc o o_n) \/ (Ts_order? (rc o o_n) (*/\ fst o < fst o_n*))) /\
                     eq (merge (do l o_n) (do s1 o_n) (do s2 o_n)) (do s3 o_n)  /\
                     eq (merge (do l o') (do s1 o') (do s2 o')) (do s3 o') /\
                     (forall k. eq_l (fst (sel_k (merge (do (do l o_n) o') (do (do s1 o_n) o') (do (do s2 o_n) o')) k))
@@ -505,7 +508,7 @@ let comm_base' (o1 o2:op_t)
           (ensures eq (merge init_st (do init_st o1) (do init_st o2)) (do (do init_st o1) o2)) = ()
 
 let comm_inter_base_right' (l s1 s2 s3:concrete_st) (o o' o1 o2:op_t) 
-  : Lemma (requires distinct_ops o o' /\ (Fst_then_snd? (rc o o') \/ (Ts_order? (rc o o') /\ fst o < fst o')) /\ 
+  : Lemma (requires distinct_ops o o' /\ (Fst_then_snd? (rc o o') \/ (Ts_order? (rc o o') (*/\ fst o < fst o'*))) /\ 
                     distinct_ops o1 o2 /\ Either? (rc o1 o2) /\
                     distinct_ops o' o1 /\ distinct_ops o' o2 /\
                     eq (merge l (do s1 o1) (do (do s2 o) o2)) (do (do (merge l s1 (do s2 o)) o1) o2) /\ //comes from comm_ind_right
@@ -519,7 +522,7 @@ let comm_inter_base_right' (l s1 s2 s3:concrete_st) (o o' o1 o2:op_t)
           (ensures eq (merge (do l o') (do (do s1 o') o1) (do (do (do s2 o) o') o2)) (do (do (do (do s3 o) o') o1) o2)) = ()
 
 let comm_inter_base_left' (l s1 s2 s3:concrete_st) (o o' o1 o2:op_t) 
-  : Lemma (requires distinct_ops o o' /\ (Fst_then_snd? (rc o o') \/ (Ts_order? (rc o o') /\ fst o < fst o')) /\ 
+  : Lemma (requires distinct_ops o o' /\ (Fst_then_snd? (rc o o') \/ (Ts_order? (rc o o') (*/\ fst o < fst o'*))) /\ 
                     distinct_ops o1 o2 /\ Either? (rc o1 o2) /\
                     distinct_ops o' o1 /\ distinct_ops o' o2 /\
                     eq (merge l (do (do s1 o) o1) (do s2 o2)) (do (do (merge l (do s1 o) s2) o1) o2) /\ //comes from comm_ind_left
@@ -559,7 +562,7 @@ let comm_inter_left' (l s1 s2 s3:concrete_st) (o1 o2 o o':op_t) (o_n:op_t{~ (com
 
 let comm_inter_lca' (l s1 s2 s3:concrete_st) (o1 o2 o:op_t)
   : Lemma (requires distinct_ops o1 o2 /\ Either? (rc o1 o2) /\ distinct_ops o1 o /\ distinct_ops o o2 /\
-                    (exists o'. Fst_then_snd? (rc o' o) \/ (Ts_order? (rc o' o) /\ fst o' < fst o)) /\
+                    (exists o'. Fst_then_snd? (rc o' o) \/ (Ts_order? (rc o' o) (*/\ fst o' < fst o*))) /\
                     eq (merge l (do s1 o1) (do s2 o2)) (do (do s3 o1) o2) /\
                     (forall k. eq_l (fst (sel_k (merge (do l o) (do (do s1 o) o1) (do (do s2 o) o2)) k))
                                (fst (sel_k (do (do (do s3 o) o1) o2) k)) /\
